
\begin{homeworkProblem}[1]
\begin{enumerate}
    \item This equation is linear.
    \[
        \begin{aligned}
        x_n &= (1-\alpha) x_{n-1} + \beta x_n \\
        (1 - \beta) x_n &= (1 - \alpha) x_{n-1} \\
        x_n &= \frac{1 - \alpha}{1 - \beta} x_{n-1}
        \end{aligned}
    \]
    \[
        \begin{aligned}
        \lambda^2 - & \frac{1 - \alpha}{1 - \beta} \lambda = 0 \\
        \lambda_1 = 0, &\quad \lambda_2 = \frac{1 - \alpha}{1 - \beta} \\
        x_n &= c(\frac{1 - \alpha}{1 - \beta})^n \\
        \end{aligned}
    \]

    \item This equation is non-linear.
    \[
        \begin{aligned}
        x_{n+1} &= \frac{x_n}{1 + x_n} \\
        x &= \frac{x}{1 + x}  \\
        x + x^2 &= x \\
        x^2 &= 0
        \end{aligned}
    \]
    x = 0 is a steady state.

    \item
\end{enumerate}
\end{homeworkProblem}