\begin{homeworkProblem}[7][(a)]

\begin{align*}
    N_{t+1} &= \lambda N_{t} e^{-aP_t}\\
    P_{t+1} &= c N_{t} (1 - e^{-aP_t})\\
\end{align*}
    Plug in $ n_t = acN_t $ and $ p_t = aP_t $ , \\
    \begin{align*}
        \frac{n_{t+1}}{ac} &= \lambda \frac{n_t}{ac} e^{-a\frac{p_t}{a}}\\
        \frac{p_{t+1}}{a} &= c\frac{n_t}{ac} (1 - e^{-a\frac{p_t}{a}}) 
    \end{align*}
    After canceling $a$ and $c$, the equations look like \begin{align*}
        n_{t+1} &= \lambda n_t e^{-p_t} \\
        p_{t+1} &= n_t (1 - e^{-p_t})
    \end{align*}
    There are only one parameter, $\lambda$, in this system of equations.
\end{homeworkProblem}
